\section{Security proof for the DMPF scheme \ref{fig:DMPF_scheme}}\label{sec_security_proof}
\subsubsection{Privacy}
\newpage
We argue the privacy of our scheme by a standard hybrid argument. 
\begin{algorithm}[H]
	\begin{algorithmic}[1]
		\caption{$Hyb_j(1^\lambda, b,A,B)$}
		\State Randomly sample $S_b^{(0)} = [s_b^{(0)}]$ from $\{0,1\}^\lambda$.
		\State Set $T_0^{(0)} = [0]$ and $T_1^{(0)} = [1]$. 
		\For{$i = 1$ to $n$}
		
		\If{$i\le j$}
		\State Randomly sample $CW^{(i)}\leftarrow \mathbb{F}^t$.
		\State Let $S_b^{(i)}$ be an empty list. 
		\State Interpret $CW^{(i)}$ as a polynomial $P_{CW^{(i)}}$.
		\For{$l = 1$ to $|A^{(i-1)}|$}
		\State Parse $map^{-1}(P_{CW^{(i)}}(map(A^{(i-1)}[l]||0^{n-i+1}))) = \Delta s||\Delta t^L||\Delta t^R$. 
		\State Parse $G(S_b^{(i-1)}[l]) = s_b^L||t_b^L||s_b^R||t_b^R$.
		\If{$A^{(i-1)}[l]||0\in A^{(i)}$ and $A^{(i-1)}[l]||1\not\in A^{(i)}$}
		\State Append $s_b^L\oplus \Delta s\cdot T_b^{(i-1)}[l]$ to $S_b^{(i)}$ and $t_b^L\oplus \Delta t^L\cdot T_b^{(i-1)}[l]$ to $T_b^{(i)}[l]$.
		\ElsIf{$A^{(i-1)}[l]||0\not\in A^{(i)}$ and $A^{(i-1)}[l]||0\in A^{(i)}$}
		\State Append $s_b^R\oplus \Delta s\cdot T_b^{(i-1)}[l]$ to $S_b^{(i)}$ and $t_b^R\oplus \Delta t^R\cdot T_b^{(i-1)}[l]$ to $T_b^{(i)}[l]$.
		\Else
		\State Append $s_b^L\oplus \Delta s\cdot T_b^{(i-1)}[l]$ to $S_b^{(i)}$ and $t_b^R\oplus \Delta t^L\cdot T_b^{(i-1)}[l]$ to $T_b^{(i)}[l]$.
		\State Append $s_b^R\oplus \Delta s\cdot T_b^{(i-1)}[l]$ to $S_b^{(i)}$ and $t_b^R\oplus \Delta t^R\cdot T_b^{(i-1)}[l]$ to $T_b^{(i)}[l]$.
		\EndIf
		\EndFor
		\Else
		\If{$i = j+1$}
		\State Sample a list $S_{1-b}^{(i-1)}$ of $|A^{(i-1)}|$ independent and random $\lambda$-bit strings.
		\State Let $T_{1-b}^{(i-1)}$ be a list such that $T_{1-b}^{(i-1)}[l] = T_{b}^{(i-1)}[l]\oplus 1$. 
		\EndIf
		\State Let $V,S_0^{(i)},T_0^{(i)}, S_1^{(i)}, T_1^{(i)}$ empty lists. 
		\For{$l = 1$ to $|A^{(i-1)}|$}
		\State Parse $G(S_b^{(i-1)}[l]) = s_b^L||t_b^L||s_b^R||t_b^R$ for $b = 0,1$. 
		\If{$A^{(i-1)}[l]||0\in A^{(i)}$ and $A^{(i-1)}[l]||1\not\in A^{(i)}$}
		\State $\Delta s||\Delta t^L||\Delta t^R\gets s_0^R\oplus s_1^R||t_0^L\oplus t_1^L\oplus 1||t_0^R\oplus t_1^R$. 
		\State Append $s_b^L\oplus \Delta s\cdot T_b^{(i-1)}[l]$ to $S_b^{(i)}$ and $t_b^L\oplus \Delta t^L\cdot T_b^{(i-1)}[l]$ to $T_b^{(i)}[l]$ for $b = 0,1$. 
		\ElsIf{$A^{(i-1)}[l]||0\not\in A^{(i)}$ and $A^{(i-1)}[l]||0\in A^{(i)}$}
		\State $\Delta s||\Delta t^L||\Delta t^R\gets s_0^L\oplus s_1^L||t_0^L\oplus t_1^L||t_0^R\oplus t_1^R\oplus 1$. 
		\State Append $s_b^R\oplus \Delta s\cdot T_b^{(i-1)}[l]$ to $S_b^{(i)}$ and $t_b^R\oplus \Delta t^R\cdot T_b^{(i-1)}[l]$ to $T_b^{(i)}[l]$ for $b = 0,1$. 
		\Else
		\State $\Delta s||\Delta t^L||\Delta t^R\gets r||t_0^L\oplus t_1^L\oplus 1||t_0^R\oplus t_1^R\oplus 1$ where $r$ is randomly sampled from $\{0,1\}^\lambda$.
		\State Append $s_b^L\oplus \Delta s\cdot T_b^{(i-1)}[l]$ to $S_b^{(i)}$ and $t_b^R\oplus \Delta t^L\cdot T_b^{(i-1)}[l]$ to $T_b^{(i)}[l]$ for $b = 0,1$. 
		\State Append $s_b^R\oplus \Delta s\cdot T_b^{(i-1)}[l]$ to $S_b^{(i)}$ and $t_b^R\oplus \Delta t^R\cdot T_b^{(i-1)}[l]$ to $T_b^{(i)}[l]$ for $b = 0,1$. 
		\EndIf
		\State Append $\Delta s||\Delta t^L||\Delta t^R$ to $V$. 
		\EndFor
		\State Let $CW^{(i)}\in \mathbb{F}^t$ be the coefficients of a $\mathbb{F}[X]$ polynomial $P_{CW}$ such that $P_{CW}(map(A^{(i-1)}[l])) = map(V[l])$ for all $1\le l\le |A^{(i-1)}|$. (If $|A^{(i-1)}|<t$ then choose $P_{CW}$ to be a random polynomial that satisfies this condition.)
		\EndIf
		
		\EndFor
		\item[]
		\Comment{Add convert layer.}
		\State Output $[S_b^{(0)}, CW^{(1)},CW^{(2)},\cdots,CW^{(n)}]$.
	\end{algorithmic}
\end{algorithm}

\begin{claim}
	Suppose $G$ is $\epsilon_G$-secure against every n.u.p.p.t. adversary, then for every $\le j\le n$, every $b\in\{0,1\}$, every $A$ containing $t$ $n$-bit strings,$B$ containing $t$ $\mathbb{G}$ elements, and every  n.u.p.p.t. adversary $Adv$, 
	\[
	|\Pr[key\leftarrow Hyb_{j-1}(1^\lambda, b, A,B), Adv(1^\lambda, key) = 1]-\Pr[key\leftarrow Hyb_{j}(1^\lambda, b, A,B), Adv(1^\lambda, key) = 1]|\le\epsilon_G|A^{(j-1)}|
	\]
\end{claim}
\begin{proof}
	Prove by contradiction. Assume $Adv$ is a n.u.p.p.t adversary that for some $1\le j\le n$, some $b\in\{0,1\}$, some $A$ and $B$,
	\[
	|\Pr[key\leftarrow Hyb_{j-1}(1^\lambda, b, A,B), Adv(1^\lambda, key) = 1]-\Pr[key\leftarrow Hyb_{j}(1^\lambda, b, A,B), Adv(1^\lambda, key) = 1]|>\epsilon_G|A^{(j-1)}|
	\]
	Then let's construct a n.u.p.p.t adversary $Adv'$ which distinguishes $\{G(s)\}^{\otimes |A^{(j-1)}|}_{s\leftarrow U(\{0,1\}^\lambda)}$ from uniform distribution with advantage larger than $\epsilon_G|A^{(j-1)}|$, which implies some PRG-adversary distinguishing $\{G(s)\}_{s\in U(\{0,1\}^\lambda)}$ uniform distribution with advantage larger than $\epsilon_G$. 
	\begin{algorithm}[H]
		\begin{algorithmic}[1]
			\caption{PRG adversary $Adv'(1^\lambda, j, b,A,B,r)$ where $r\in\{0,1\}^{(2\lambda+2)|A^{(j-1)}|}$ is the challenge}
			\State Parse $r = r^1_0||r^1_1||r^2_0||r^2_1||\cdots||r^{|A^{(j-1)}|}_0||r^{|A^{(j-1)}|}_1$ where $|r^l_z| = \lambda+1$.
			\State Randomly sample $S_b^{(0)} = [s_b^{(0)}]$ from $\{0,1\}^\lambda$.
			\State Set $T_0^{(0)} = [0]$ and $T_1^{(0)} = [1]$. 
			\For{$i = 1$ to $n$}
			
			\If{$i\le j-1$}
			\State Randomly sample $CW^{(i)}\leftarrow \mathbb{F}^t$.
			\State Let $S_b^{(i)}$ be an empty list. 
			\State Interpret $CW^{(i)}$ as a polynomial $P_{CW^{(i)}}$.
			\For{$l = 1$ to $|A^{(i-1)}|$}
			\State Parse $map^{-1}(P_{CW^{(i)}}(map(A^{(i-1)}[l]||0^{n-i+1}))) = \Delta s||\Delta t^L||\Delta t^R$. 
			\State Parse $G(S_b^{(i-1)}[l]) = s_b^L||t_b^L||s_b^R||t_b^R$.
			\If{$A^{(i-1)}[l]||0\in A^{(i)}$ and $A^{(i-1)}[l]||1\not\in A^{(i)}$}
			\State Append $s_b^L\oplus \Delta s\cdot T_b^{(i-1)}[l]$ to $S_b^{(i)}$ and $t_b^L\oplus \Delta t^L\cdot T_b^{(i-1)}[l]$ to $T_b^{(i)}[l]$.
			\ElsIf{$A^{(i-1)}[l]||0\not\in A^{(i)}$ and $A^{(i-1)}[l]||0\in A^{(i)}$}
			\State Append $s_b^R\oplus \Delta s\cdot T_b^{(i-1)}[l]$ to $S_b^{(i)}$ and $t_b^R\oplus \Delta t^R\cdot T_b^{(i-1)}[l]$ to $T_b^{(i)}[l]$.
			\Else
			\State Append $s_b^L\oplus \Delta s\cdot T_b^{(i-1)}[l]$ to $S_b^{(i)}$ and $t_b^R\oplus \Delta t^L\cdot T_b^{(i-1)}[l]$ to $T_b^{(i)}[l]$.
			\State Append $s_b^R\oplus \Delta s\cdot T_b^{(i-1)}[l]$ to $S_b^{(i)}$ and $t_b^R\oplus \Delta t^R\cdot T_b^{(i-1)}[l]$ to $T_b^{(i)}[l]$.
			\EndIf
			\EndFor
			\Else
			\State Define $R_0^l||R_1^l = \begin{cases}r_0^l||r_1^l & i = j\\G(S_{1-b}^{(i-1)}[l]) & \text{else}\end{cases}$ for $1\le l\le |A^{(i-1)}|$.
			\State Let $V,S_0^{(i)},T_0^{(i)}, S_1^{(i)}, T_1^{(i)}$ empty lists. 
			\For{$l = 1$ to $|A^{(i-1)}|$}
			\State Parse $G(S_b^{(i-1)}[l]) = s_b^L||t_b^L||s_b^R||t_b^R$.
			\State Parse $R_0^l||R_1^l = s_{1-b}^L||t_{1-b}^L||s_{1-b}^R||t_{1-b}^R$.
			\If{$A^{(i-1)}[l]||0\in A^{(i)}$ and $A^{(i-1)}[l]||1\not\in A^{(i)}$}
			\State $\Delta s||\Delta t^L||\Delta t^R\gets s_0^R\oplus s_1^R||t_0^L\oplus t_1^L\oplus 1||t_0^R\oplus t_1^R$. 
			\State Append $s_b^L\oplus \Delta s\cdot T_b^{(i-1)}[l]$ to $S_b^{(i)}$ and $t_b^L\oplus \Delta t^L\cdot T_b^{(i-1)}[l]$ to $T_b^{(i)}[l]$ for $b = 0,1$. 
			\ElsIf{$A^{(i-1)}[l]||0\not\in A^{(i)}$ and $A^{(i-1)}[l]||0\in A^{(i)}$}
			\State $\Delta s||\Delta t^L||\Delta t^R\gets s_0^L\oplus s_1^L||t_0^L\oplus t_1^L||t_0^R\oplus t_1^R\oplus 1$. 
			\State Append $s_b^R\oplus \Delta s\cdot T_b^{(i-1)}[l]$ to $S_b^{(i)}$ and $t_b^R\oplus \Delta t^R\cdot T_b^{(i-1)}[l]$ to $T_b^{(i)}[l]$ for $b = 0,1$. 
			\Else
			\State $\Delta s||\Delta t^L||\Delta t^R\gets r||t_0^L\oplus t_1^L\oplus 1||t_0^R\oplus t_1^R\oplus 1$ where $r$ is randomly sampled from $\{0,1\}^\lambda$.
			\State Append $s_b^L\oplus \Delta s\cdot T_b^{(i-1)}[l]$ to $S_b^{(i)}$ and $t_b^R\oplus \Delta t^L\cdot T_b^{(i-1)}[l]$ to $T_b^{(i)}[l]$ for $b = 0,1$. 
			\State Append $s_b^R\oplus \Delta s\cdot T_b^{(i-1)}[l]$ to $S_b^{(i)}$ and $t_b^R\oplus \Delta t^R\cdot T_b^{(i-1)}[l]$ to $T_b^{(i)}[l]$ for $b = 0,1$. 
			\EndIf
			\State Append $\Delta s||\Delta t^L||\Delta t^R$ to $V$. 
			\EndFor
			\State Let $CW^{(i)}\in \mathbb{F}^t$ be the coefficients of a $\mathbb{F}[X]$ polynomial $P_{CW}$ such that $P_{CW}(map(A^{(i-1)}[l])) = map(V[l])$ for all $1\le l\le |A^{(i-1)}|$. (If $|A^{(i-1)}|<t$ then choose $P_{CW}$ to be a random polynomial that satisfies this condition.)
			\EndIf
			\EndFor
			
			\item[]
			\Comment{Add convert layer.}
			\State $key \gets [S_b^{(0)}, CW^{(1)},CW^{(2)},\cdots,CW^{(n)}]$
			\State Output $Adv(1^\lambda,key)$. 
		\end{algorithmic}
	\end{algorithm}
	
	If $r$ is a sample of $\{G(s)\}^{\otimes |A^{(j-1)}|}_{s\in U(\{0,1\}^\lambda}$, then $r^l_0||r^l_1 = G(s^l)$ for some randomly sampled $s^l$, for all $1\le l\le |A^{(j-1)}|$, which generates $key$ in the same way as $Hyb_{j-1}$.  Meanwhile if $r$ is from the uniform distribution, the procedure generates $key$ in the same way as $Hyb_j$. 
	
	Hence,
	\begin{align*}
		&|\Pr[key\leftarrow Hyb_{j-1}(1^\lambda, b, A,B), Adv(1^\lambda, key) = 1]-\Pr[key\leftarrow Hyb_{j}(1^\lambda, b, A,B), Adv(1^\lambda, key) = 1]|\\
		=&|\Pr[s\leftarrow U(\{0,1\}^{\lambda|A^{(j-1)}|}) , Adv'(1^\lambda, j, b,A,B,G^{\otimes |A^{(j-1)}|}(s) = 1] - \Pr[r\leftarrow U(\{0,1\}^{(2\lambda+2)|A^{(j-1)}|}), Adv'(1^\lambda, j, b,A,B,r) = 1]| \\
		\le & \epsilon_G|A^{(j-1)}|
	\end{align*} 
\end{proof}
Together with the following two facts: 
\begin{enumerate}
	\item $\{key\leftarrow Hyb_0(1^\lambda, b, A,B)\} = \{k_b | (k_0,k_1)\leftarrow Gen(1^\lambda, A,B)\}$
	\item $\{key\leftarrow Hyb_{n}(1^\lambda, b, A,B)\}$ is truly random. 
\end{enumerate}
we have the following security of the DMPF scheme:
\begin{theorem}
	Suppose $G:\{0,1\}^\lambda\rightarrow\{0,1\}^{2\lambda+2}$ is $\epsilon_G$-secure against every n.u.p.p.t. adversary. Then the scheme is a secure distributed $t$-point function scheme for the function family $f_{A,B}:\{0,1\}^n\rightarrow \mathbb{G}$ with key size $tn(\lambda+1) +\lambda keysize_{convert}$ with secrecy $tn\epsilon_G+\epsilon_{convert}$.
\end{theorem}